src/Extraction/Extraction.v
@@ -1,53 +1,83 @@
 From Coq Require Extraction.
 Require Import ExtrHaskellBasic.
-Require Import ExtrHaskellNatInteger.
+(* Require Import ExtrHaskellNatInteger. *)
+(** This is dangerous since Int is bounded, unlike Integer.
+    Leaves the code open to overflows. Until I find a better alternative,
+    this is the hacky way to go. **)
+Require Import ExtrHaskellNatInt. 
 Require Import ExtrHaskellZInteger.
 Require Import ExtrHaskellString.
+
 Extraction Language Haskell.
 
 Require Import Framework FSParameters.
 Require LogCache Transaction File.
 
-Cd "./Extracted".
-Extract Inlined Constant addr => "Prelude.Integer".
-Extract Constant user => "System.Posix.Types.UserID".
-Extract Constant value => "Prelude.Int".
-Extract Constant file_blocks_count => "4096". (* 4K data blocks *)
-Extract Constant log_length => "500". (* 500 log blocks *)
-Extract Constant inode_count => "4096". (* 4K inodes *)
-Extract Constant disk_size => "4 Prelude.* 1024 Prelude.* 1024 Prelude.* 1024". (* 4 GB disk *)
 
-(* Eliminate Horizontal Composition *) 
+Extract Constant addr => "Prelude.Int".
+Extract Inlined Constant addr_eq_dec => "(Prelude.==)".
+
+Extract Constant user => "System.Posix.Types.UserID".
+Extract Constant value => "Prelude.Int". (** We need to change this but to what? **)
+Extract Constant block_size => "8 Prelude.* 4096". (** 4KB blocks **) 
+Extract Constant file_blocks_count => "4096". (** 4K data blocks *)
+Extract Constant log_length => "500". (** 500 log blocks *)
+Extract Constant inode_count => "4096". (** 4K inodes *)
+Extract Constant disk_size => "4 Prelude.* 1024 Prelude.* 1024 Prelude.* 1024". (** 4 GB disk *)
+
+(** These need to be defined as well
+Extract Constant BlockAllocator.bits_to_value => "".
+Extract Constant BlockAllocator.value_to_bits => "".
+
+Extract Constant addr_list_to_blocks => "".
+Extract Constant blocks_to_addr_list => "".
+
+Extract Constant Log.encode_header => "".
+Extract Constant Log.decode_header => "".
+
+Extract Constant hash => "".
+Extract Inline Constant hash_eq_dec => "".
+Extract Inline Constant hash0 => "".
+
+Extract Constant key => "".
+Extract Constant Inode.encode_inode => "".
+Extract Constant Inode.decode_inode => "".
+**)
+
+(** Eliminate Horizontal Composition **) 
 Extraction Implicit lift_L1 [ 1 2 ].
 Extraction Implicit lift_L2 [ 1 2 ]. 
 Extract Inlined Constant lift_L1 => "".
 Extract Inlined Constant lift_L2 => "".
 
-Extraction Inline Operation.prog.
+Extraction Inline Core.operation.
 Extraction Inline Language.prog. 
 
 Extract Inductive Language.prog' => "Prelude.IO" [ "" "Prelude.return" "(Prelude.>>=)" ].
 
-(* Use these to implement actual functionality
+(** Use these to implement actual functionality 
 Extract Inductive DiskLayer.disk_prog => "Prelude.IO" [ "DISK_READ" "DISK_WRITE" "DISK_SYNC" ].
 Extract Inductive CryptoLayer.crypto_prog => "Prelude.IO" [ "GET_KEY" "HASH" "ENCRYPT" "DECRYPT" ].
 Extract Inductive CacheLayer.cache_prog => "Prelude.IO" [ "CACHE_READ" "CACHE_WRITE" "CACHE_FLUSH"]. 
-Extract Inductive StorageLayer.storage_prog => "Prelude.IO" [ "GET" "PUT" "DELETE" ].
- *)
+Extract Inductive ListLayer.list_prog => "Prelude.IO" [ "GET" "PUT" "DELETE" ].
+*)
 
 Extract Inductive AuthenticationLayer.authentication_prog => "Prelude.IO" [ "(\u -> do uid <- System.Posix.User.getEffectiveUserID; Prelude.return (u Prelude.== uid))" ].
 
-Extract Inductive LoggedDiskLayer.logged_disk_prog => "Prelude.IO" [ "LogCache.read" "LogCache.write" ].
-Extract Inductive TransactionalDiskLayer.transactional_disk_prog => "Prelude.IO" [ "Transaction.start" "Transaction.read" "Transaction.write" "Transaction.commit" "Transaction.abort" ].
+Extract Inductive LoggedDiskLayer.logged_disk_prog => "Prelude.IO" [ "LogCache.read" "LogCache.write" "LogCache.recover" "LogCache.init" ].
+Extract Inductive TransactionalDiskLayer.transactional_disk_prog => "Prelude.IO" [ "Transaction.read" "Transaction.write" "Transaction.commit" "Transaction.abort" "Transaction.recover" "Transaction.init" ].
 
 Separate Extraction
            File.read File.write
            File.change_owner File.extend
            File.delete File.create
-           Transaction.start Transaction.read
+           File.recover File.init
+           Transaction.read
            Transaction.write Transaction.commit
            Transaction.abort
-           LogCache.read LogCache.write.
+           Transaction.recover Transaction.init
+           LogCache.read LogCache.write
+           LogCache.recover LogCache.init.
 
 
-(* Run compile.sh now *)
+(** Run compile.sh now *)
