src/Extraction/compile.sh
@@ -1,14 +1,9 @@
 #! /bin/bash
 
-# Recreate extraction directory
-# rm -rf Extracted
-# mkdir Extracted
-
-# Run extraction
-# dune build Extraction.v
-
-
-cd ./Extracted
+rm -rf ./extracted
+mkdir extracted
+mv ./*.hs ./extracted
+cd extracted
 
 # Write imports to proper files
 sed -ie '/^module/a import qualified LogCache' Transaction.hs
@@ -18,4 +13,4 @@ sed -ie '/^module/a import qualified System.Posix.User' File.hs
 sed -ie '/^module/a import qualified System.Posix.Types' BaseTypes.hs
 
 # Compile Haskell files 
-ghc *.hs
+ghc File.hs
